locality
git-svn-id: svn://scm.gforge.inria.fr/svn/cfml@96 ba02c806-7d2b-4818-9a48-35b22e6bdc79

CFHeaps.v
@@ -6,21 +6,37 @@ Require Export LibCore LibEpsilon Shared LibMap.
 (* ** Heaps *)
 
 (*------------------------------------------------------------------*)
+(* ** Representation of values packed with their type *)
+
+(** Representation of heap items *)
+
+Record dynamic := dyn { 
+  dyn_type : Type; 
+  dyn_value : dyn_type }.
+
+Lemma dyn_inj : forall A (x y : A),
+  dyn x = dyn y -> x = y. 
+Proof. introv H. inverts~ H. Qed.
+
+Lemma dyn_inj_type : forall A1 A2 (x1:A1) (x2:A2),
+  dyn x1 = dyn x2 -> A1 = A2.
+Proof. introv H. inverts~ H. Qed.
+
+Lemma dyn_eta : forall d, 
+  d = dyn (dyn_value d).
+Proof. intros. destruct~ d. Qed.
+
+
+(*------------------------------------------------------------------*)
 (* ** Representation of heaps *)
 
 (** Representation of locations *)
 
 Definition loc : Type := nat.
 
-(** Representation of heap items *)
-
-Record dyn := { 
-  dyn_type : Type; 
-  dyn_value : dyn_type }.
-
 (** Representation of heaps *)
 
-Definition heap := option (map loc dyn).
+Definition heap := option (map loc dynamic).
 
 (*------------------------------------------------------------------*)
 (* ** Construction of heaps *)
@@ -33,7 +49,7 @@ Definition heap_empty : heap :=
 (** Singleton heap *)
 
 Definition heap_single (l:loc) A (v:A) : heap := 
-  Some (single_bind l (Build_dyn v)).
+  Some (single_bind l (dyn v)).
 
 (** Heap union *)
 
@@ -99,7 +115,7 @@ Notation "[ L ]" := (heap_is_empty_st L)
 Notation "\[ P ]" := (fun v => heap_is_empty_st (P v)) 
   (at level 0, P at level 99) : heap_scope.
 
-Notation "H1 '**' H2" := (heap_is_star H1 H2)
+Notation "H1 '\*' H2" := (heap_is_star H1 H2)
   (at level 40, left associativity) : heap_scope.
 Notation "H1 '*' H2" := (heap_is_star H1 H2)
   (at level 40, left associativity, only parsing) : heap_scope.
@@ -113,9 +129,11 @@ Notation "l '~>' v" := (heap_is_single l (=v))
 Notation "'Hexists' x , H" := (heap_is_pack (fun x => H))
   (at level 35, x ident, H at level 200) : heap_scope.
 
-Notation "Q *** H" := (starpost Q H) (at level 40).
+Notation "Q \*+ H" := (starpost Q H) (at level 40).
 
 Open Scope heap_scope.
+Bind Scope heap_scope with hprop.
+Delimit Scope heap_scope with h.
 
 
 (*------------------------------------------------------------------*)
@@ -134,7 +152,7 @@ Lemma star_assoc : LibOperation.assoc heap_is_star.
 Proof. skip. Qed.
 
 Lemma starpost_neutral : forall B (Q:B->hprop),
-  Q *** [] = Q.
+  Q \*+ [] = Q.
 Proof. extens. intros. unfold starpost. rewrite~ star_neutral_r. Qed.
 
 
@@ -168,6 +186,21 @@ Tactic Notation "rew_heap" "*" "in" hyp(H) :=
 
 
 
+
+(* todo: move *)
+
+Lemma rel_le_refl : forall A B (P:A->B->Prop),
+  rel_le P P.
+Proof. intros_all~. Qed.
+Hint Resolve rel_le_refl.
+
+Lemma heap_weaken_star : forall H1' H1 H2 H3,
+  (H1 ==> H1') -> (H1' * H2 ==> H3) -> (H1 * H2 ==> H3).
+Proof.
+  introv W M (h1&h2&N). intuit N. apply M. exists~ h1 h2.
+Qed.
+
+
 (********************************************************************)
 (* ** Locality *)
 
@@ -183,175 +216,10 @@ Notation "'~~' B" := (hprop->(B->hprop)->Prop)
 
 Definition local B (F:~~B) : ~~B :=
   fun (H:hprop) (Q:B->hprop) =>
-    exists H1 H2 Q1 H',
-       H ==> H1 * H2
-    /\ (forall h, H1 h -> exists H1', H1' h /\ F H1' Q1)
-    /\ forall x, (Q1 x) * H2 ==> (Q x) * H'.
-
-(** Characterization of "local" judgments *)
-
-Definition is_local B (F:~~B) :=
-  F = local F.
-
-(** The weakening property is implied by locality *)
-
-Definition weakenable B (F:~~B) :=
-  forall H Q , F H Q ->
-  forall H' Q', H' ==> H -> Q ===> Q' -> F H' Q'.
-
-
-Lemma local_intro_exists : forall B (F:~~B) H1 H2 A (J:A->hprop) Q,
-  is_local F -> (forall x, F (H1 * (J x) * H2) Q) ->
-   F (H1 * heap_is_pack J * H2) Q.
-Proof.
-  introv L M. rewrite L.
-  exists (H1 * heap_is_pack J * H2) [] Q []. splits.
-  skip. (* heaps *)
-  intros. intuit H. intuit H3. intuit H7.
-  specializes M x3. subst x h. esplit. split; [| apply M].
-  exists __ __. splits. eauto. eauto. 
-  exists __ __. splits. eauto. eauto. eauto. eauto. eauto.  
-  auto.
-Qed. 
-
-
-(*------------------------------------------------------------------*)
-(* ** Properties of [local] *)
-
-(** The [local] operator can be freely erased from a conclusion *)
-
-Lemma local_erase : forall B (F:~~B), 
-  forall H Q, F H Q -> local F H Q.
-Proof.
-  intros. exists H [] Q []. splits.
-  rew_heap~. auto.
-intros. exists H. split~.
-auto.
-Qed.
-
-
-(** Nested applications [local] are redundant *)
-
-Lemma local_local : forall B (F:~~B),
-  local (local F) = local F.
-Proof.
-  extens. intros H Q. iff M. 
-  destruct M as (H1&H2&Q1&H'&?&N&?).
-  destruct N as (H1'&H2'&Q1'&H''&?&?&?).
-  exists H1' (H2 ** H2') Q1' (H' ** H''). splits.
-  eapply pred_le_trans. eauto.
-   intros h Hh. hnf in Hh. destruct Hh as (h1&h2&?&?&?&?).
-   subst h. applys_to H9 H4. intuit H9. subst h1.
-   rewrite (star_comm H2). rewrite star_assoc.
-   exists __ __. splits~. exists __ __. splits~.
-  eauto.
-  intros.
-  skip. (* todo *)
-  apply~ local_erase.
-Qed.
-
-(** A definition whose head is [local] satisfies [is_local] *)
-
-Lemma local_is_local : forall B (F:~~B),
-  is_local (local F).
-Proof. intros. unfolds. rewrite~ local_local. Qed.
-*)
-
-(** Elimination lemma associated with the definition of [local] *)
-
-Lemma local_elim : forall B (F:~~B) H H1 H2 H' Q1 Q,
-  is_local F -> 
-  F H1 Q1 -> 
-  H ==> H1 ** H2 -> 
-  Q1 *** H2 ===> Q *** H' ->
-  F H Q.
-Proof.
-  introv L M WH WQ. rewrite L. exists H1 H2 Q1 H'. splits.
-  auto. auto. intros. rew_heap~. apply WQ.
-Qed.
-
-(** Corrolary for the case where no garbage collection is required *)
-
-Lemma local_frame : forall B (F:~~B) H H1 H2 Q1 Q,
-  is_local F -> 
-  F H1 Q1 -> 
-  H ==> H1 ** H2 -> 
-  Q1 *** H2 ===> Q ->
-  F H Q.
-Proof.
-  intros. eapply local_elim with (H' := []); eauto. rew_heap~.
-Qed.
-
-(** Corrolary for the case where no frame is required *)
-
-Lemma local_weaken : forall B (F:~~B) H H' Q Q',
-  is_local F -> 
-  F H' Q' -> 
-  H ==> H' -> 
-  Q' ===> Q ->
-  F H Q.
-Proof.
-  intros. eapply local_frame with (H2 := []); eauto; rew_heap~.
-Qed.
-
-Lemma local_weaken' : forall B (F:~~B),
-  is_local F -> weakenable F.
-Proof. intros_all. apply* local_weaken. Qed.
-  (* todo: use only one lemma *)
-
-
-Definition local' B (F:~~B) : ~~B :=
-  fun (H:hprop) (Q:B->hprop) =>
-    exists H1 H2 P Q1 H',
-       H ==> H1 * H2 * [P]
-    /\ (P -> F H1 Q1)
-    /\ forall x, (Q1 x) * H2 ==> (Q x) * H'.
-
-Lemma local_intro_prop : forall B (F:~~B) H1 H2 (P:Prop) Q,
-  is_local F -> (P -> F (H1 * H2) Q) -> F (H1 * [P] * H2) Q.
-Proof.
-  introv L M. rewrite L.
-  skip_rewrite (local = local').
-  exists (H1 * H2) [] P Q []. splits.
-  skip. (* heaps *)
-  auto.
-  auto.
-Qed. 
-
-Lemma local_intro_exists : forall B (F:~~B) H1 H2 A (J:A->hprop) Q,
-  is_local F -> (forall x, F (H1 * (J x) * H2) Q) ->
-   F (H1 * heap_is_pack J * H2) Q.
-Proof.
-  introv L M. rewrite L.
-  skip_rewrite (local = local').
-  exists (H1 * H2) [] True Q []. splits.
-  skip. (* heaps *)
-  auto.
-  auto.
-Qed. 
-
-
-
-f
-(********************************************************************)
-(* ** Locality *)
-
-(*------------------------------------------------------------------*)
-(* ** Definition of [local] *)
-
-(** Type of post-conditions on values of type B *)
-
-Notation "'~~' B" := (hprop->(B->hprop)->Prop) 
-  (at level 8, only parsing) : type_scope.
-
-(** "Local" = Frame rule + consequence rule + garbage collection *)
-
-Definition local B (F:~~B) : ~~B :=
-  fun (H:hprop) (Q:B->hprop) =>
-    exists H1 H2 Q1 H',
-       H ==> H1 * H2
+    forall h, H h -> exists H1 H2 Q1 H',
+       (H1 \* H2) h 
     /\ F H1 Q1
-    /\ forall x, (Q1 x) * H2 ==> (Q x) * H'.
+    /\ Q1 \*+ H2 ===> Q \*+ H'.
 
 (** Characterization of "local" judgments *)
 
@@ -383,17 +251,18 @@ Lemma local_local : forall B (F:~~B),
   local (local F) = local F.
 Proof.
   extens. intros H Q. iff M. 
-  destruct M as (H1&H2&Q1&H'&?&N&?).
-  destruct N as (H1'&H2'&Q1'&H''&?&?&?).
-  exists H1' (H2 ** H2') Q1' (H' ** H''). splits.
-  eapply pred_le_trans. eauto.
-   intros h Hh. hnf in Hh. destruct Hh as (h1&h2&?&?&?&?).
-   subst h. applys_to H9 H4. intuit H9. subst h1.
-   rewrite (star_comm H2). rewrite star_assoc.
-   exists __ __. splits~. exists __ __. splits~.
-  eauto.
-  intros.
-  skip. (* todo *)
+  introv PH.
+  destruct (M _ PH) as (H1&H2&Q1&H'&PH12&N&Qle).
+  destruct PH12 as (h1&h2&Ph12&Fh12&PH1&PH2).
+  destruct (N _ PH1) as (H1'&H2'&Q1'&H''&PH12'&N'&Qle').
+  exists H1' (H2' \* H2) Q1' (H' \* H''). splits.
+   rewrite star_assoc.
+   exists~ h1 h2.
+   auto.
+   intros x. specializes Qle x. specializes Qle' x. unfolds starpost.
+    rewrite star_assoc. applys heap_weaken_star Qle'.
+    rewrite (star_assoc (Q x)). 
+    skip_cuts (Q1 x \* H2 ==> Q x \* H'). auto.
   apply~ local_erase.
 Qed.
 
@@ -403,75 +272,81 @@ Lemma local_is_local : forall B (F:~~B),
   is_local (local F).
 Proof. intros. unfolds. rewrite~ local_local. Qed.
 
-(** Elimination lemma associated with the definition of [local] *)
+(** Weaken and frame and gc property [local] *)
 
-Lemma local_elim : forall B (F:~~B) H H1 H2 H' Q1 Q,
+Lemma local_wgframe : forall B (F:~~B) H H1 H2 H' Q1 Q,
   is_local F -> 
   F H1 Q1 -> 
-  H ==> H1 ** H2 -> 
-  Q1 *** H2 ===> Q *** H' ->
+  H ==> H1 \* H2 -> 
+  Q1 \*+ H2 ===> Q \*+ H' ->
   F H Q.
 Proof.
-  introv L M WH WQ. rewrite L. exists H1 H2 Q1 H'. splits.
-  auto. auto. intros. rew_heap~. apply WQ.
+  introv L M WH WQ. rewrite L. introv Ph.
+  exists H1 H2 Q1 H'. splits; rew_heap~.
 Qed.
 
-(** Corrolary for the case where no garbage collection is required *)
+(** Weaken and frame properties from [local] *)
 
-Lemma local_frame : forall B (F:~~B) H H1 H2 Q1 Q,
+Lemma local_wframe : forall B H1 H2 Q1 (F:~~B) H Q,
   is_local F -> 
   F H1 Q1 -> 
-  H ==> H1 ** H2 -> 
-  Q1 *** H2 ===> Q ->
+  H ==> H1 \* H2 -> 
+  Q1 \*+ H2 ===> Q ->
   F H Q.
 Proof.
-  intros. eapply local_elim with (H' := []); eauto. rew_heap~.
+  introv L M WH WQ. rewrite L. introv Ph.
+  exists H1 H2 Q1 []. splits; rew_heap~.
 Qed.
 
-(** Corrolary for the case where no frame is required *)
+(** Weakening from [local] *)
 
-Lemma local_weaken : forall B (F:~~B) H H' Q Q',
+Lemma local_weaken : forall B H' Q' (F:~~B) H Q,
   is_local F -> 
   F H' Q' -> 
   H ==> H' -> 
   Q' ===> Q ->
   F H Q.
 Proof.
-  intros. eapply local_frame with (H2 := []); eauto; rew_heap~.
+  intros. eapply local_wframe with (H2 := []); eauto; rew_heap~.
 Qed.
 
 Lemma local_weaken' : forall B (F:~~B),
   is_local F -> weakenable F.
 Proof. intros_all. apply* local_weaken. Qed.
-  (* todo: use only one lemma *)
+    (* todo: use only one lemma *)
 
+(** Garbage collection from [local] *)
 
-Definition local' B (F:~~B) : ~~B :=
-  fun (H:hprop) (Q:B->hprop) =>
-    exists H1 H2 P Q1 H',
-       H ==> H1 * H2 * [P]
-    /\ (P -> F H1 Q1)
-    /\ forall x, (Q1 x) * H2 ==> (Q x) * H'.
-
-Lemma local_intro_prop : forall B (F:~~B) H1 H2 (P:Prop) Q,
-  is_local F -> (P -> F (H1 * H2) Q) -> F (H1 * [P] * H2) Q.
+Lemma local_gc : forall B H' Q' (F:~~B) H Q,
+  is_local F -> 
+  F H Q' ->
+  Q' ===> Q \*+ H' ->
+  F H Q.
 Proof.
-  introv L M. rewrite L.
-  skip_rewrite (local = local').
-  exists (H1 * H2) [] P Q []. splits.
-  skip. (* heaps *)
-  auto.
-  auto.
+  introv L M W. rewrite L. introv Ph.
+  exists H [] Q' H'. splits; rew_heap~.
+Qed.
+
+(** Extraction of premisses from [local] *)
+
+Lemma local_intro_prop : forall B (F:~~B) H (P:Prop) Q,
+  is_local F -> (P -> F H Q) -> F ([P] * H) Q.
+Proof.
+  introv L M. rewrite L. introv (h1&h2&?&?&(PH1&HP)&PH2).
+  skip: (h = h2). (* todo heaps *) subst h2.
+  exists H [] Q []. splits; rew_heap~.
 Qed. 
 
-Lemma local_intro_exists : forall B (F:~~B) H1 H2 A (J:A->hprop) Q,
-  is_local F -> (forall x, F (H1 * (J x) * H2) Q) ->
-   F (H1 * heap_is_pack J * H2) Q.
+(** Extraction of existential from [local] *)
+
+Lemma local_intro_exists : forall B (F:~~B) H A (J:A->hprop) Q,
+  is_local F -> 
+  (forall x, F ((J x) * H) Q) ->
+   F (heap_is_pack J * H) Q.
 Proof.
-  introv L M. rewrite L.
-  skip_rewrite (local = local').
-  exists (H1 * H2) [] True Q []. splits.
-  skip. (* heaps *)
+  introv L M. rewrite L. introv (h1&h2&?&?&(X&HX)&PH2).
+  exists (J X * H) [] Q []. splits.
+  rew_heap~. exists~ h1 h2.
   auto.
   auto.
 Qed. 
